{-# OPTIONS --safe #-}
module Data.AF.Examples where

open import Foundations.Base
open import Foundations.HLevel
open import Data.Empty.Base
open import Data.Unit.Base
open import Data.Bool.Base as Bool
open import Data.Dec.Base as Dec
open import Data.Reflects.Base
open import Data.Sum.Base
open import Data.Sum.Path
open import Data.Maybe.Base
open import Data.List.Base
open import Data.AF.Base
open import Data.AF.Ramsey
open import Data.AF.WF
open import Data.AF.Constructions
open import Data.Acc.Base
open import Data.Nat
open import Data.Nat.Order.Base
open import Data.Star.Base
open import Data.Plus.Base
open import Data.Plus.Properties

private variable
  â„“ â„“â€² â„“â€³ : Level
  A B : ğ’° â„“
  R T : A â†’ A â†’ ğ’° â„“â€²

-- flex

Tfl : â„• Ã— â„• â†’ â„• Ã— â„• â†’ ğ’°
Tfl (xâ‚ , xâ‚‚) (yâ‚ , yâ‚‚) = (xâ‚ < yâ‚) âŠ ((xâ‚ ï¼ yâ‚) Ã— (xâ‚‚ < yâ‚‚))

Rfl : â„• Ã— â„• â†’ â„• Ã— â„• â†’ ğ’°
Rfl (xâ‚ , xâ‚‚) (yâ‚ , yâ‚‚) = (xâ‚ â‰¤ yâ‚) Ã— (xâ‚‚ â‰¤ yâ‚‚)

Tfl-trans : âˆ€ {xâ‚ xâ‚‚ yâ‚ yâ‚‚ zâ‚ zâ‚‚}
          â†’ Tfl (xâ‚ , xâ‚‚) (yâ‚ , yâ‚‚)
          â†’ Tfl (yâ‚ , yâ‚‚) (zâ‚ , zâ‚‚)
          â†’ Tfl (xâ‚ , xâ‚‚) (zâ‚ , zâ‚‚)
Tfl-trans (inl xâ‚<yâ‚)            (inl yâ‚<zâ‚)           = inl (<-trans xâ‚<yâ‚ yâ‚<zâ‚)
Tfl-trans (inl xâ‚<yâ‚)            (inr (yâ‚=zâ‚ , yâ‚‚<zâ‚‚)) = inl (<-â‰¤-trans xâ‚<yâ‚ (=â†’â‰¤ yâ‚=zâ‚))
Tfl-trans (inr (xâ‚=yâ‚ , xâ‚‚<yâ‚‚))  (inl yâ‚<zâ‚)           = inl (â‰¤-<-trans (=â†’â‰¤ xâ‚=yâ‚) yâ‚<zâ‚)
Tfl-trans (inr (xâ‚=yâ‚ , xâ‚‚<yâ‚‚))  (inr (yâ‚=zâ‚ , yâ‚‚<zâ‚‚)) = inr ((xâ‚=yâ‚ âˆ™ yâ‚=zâ‚) , (<-trans xâ‚‚<yâ‚‚ yâ‚‚<zâ‚‚))

Tfl-empty-intersect : âˆ€ {xâ‚ xâ‚‚ yâ‚ yâ‚‚}
                    â†’ Plus Tfl (xâ‚ , xâ‚‚) (yâ‚ , yâ‚‚)
                    â†’ Rfl (yâ‚ , yâ‚‚) (xâ‚ , xâ‚‚)
                    â†’ âŠ¥
Tfl-empty-intersect p (yâ‚â‰¤xâ‚ , yâ‚‚â‰¤xâ‚‚) =
  [ (Î» xâ‚<yâ‚ â†’ <â†’â‰± xâ‚<yâ‚ yâ‚â‰¤xâ‚)
  , (Î» where (_ , xâ‚‚<yâ‚‚) â†’ <â†’â‰± xâ‚‚<yâ‚‚ yâ‚‚â‰¤xâ‚‚)
  ]áµ¤ (plus-fold1 (record { _âˆ™_ = Tfl-trans }) p)

-- or directly by induction
Tfl-empty-intersectâ€² : âˆ€ {xâ‚ xâ‚‚ yâ‚ yâ‚‚}
                    â†’ Plus Tfl (xâ‚ , xâ‚‚) (yâ‚ , yâ‚‚)
                    â†’ Rfl (yâ‚ , yâ‚‚) (xâ‚ , xâ‚‚)
                    â†’ âŠ¥
Tfl-empty-intersectâ€² [ inl x<yâ‚ ]âº       (yâ‰¤xâ‚ , yâ‰¤xâ‚‚) = <â†’â‰± x<yâ‚ yâ‰¤xâ‚
Tfl-empty-intersectâ€² [ inr (e , x<yâ‚‚) ]âº (yâ‰¤xâ‚ , yâ‰¤xâ‚‚) = <â†’â‰± x<yâ‚‚ yâ‰¤xâ‚‚
Tfl-empty-intersectâ€² (h â—…âº p)            (yâ‰¤xâ‚ , yâ‰¤xâ‚‚) =
  [ â‰¤â†’â‰¯ (plus-fold1 Trans-â‰¤ (plus-map [ <â†’â‰¤ , =â†’â‰¤ âˆ˜ fst ]áµ¤ p) âˆ™ yâ‰¤xâ‚)
  , (Î» where (e , x<wâ‚‚) â†’ Tfl-empty-intersectâ€² p (yâ‰¤xâ‚ âˆ™ =â†’â‰¤ e , yâ‰¤xâ‚‚ âˆ™ <â†’â‰¤ x<wâ‚‚))
  ]áµ¤ h

flex : â„• Ã— â„• â†’ â„•
flex =
  to-induction
    (AFâ†’WF (af-Ã— af-â‰¤ af-â‰¤) Tfl-empty-intersect)
    (Î» _ â†’ â„•)
    Î» x ih â†’ go (x .fst) (x .snd) Î» a b â†’ ih (a , b)
  where
  go : âˆ€ x y â†’ (âˆ€ a b â†’ Tfl (a , b) (x , y) â†’ â„•) â†’ â„•
  go  zero    _      _  = 1
  go (suc _)  zero   _  = 1
  go (suc x) (suc y) ih = ih x (2 + y) (inl <-ascend) + ih (1 + x) y (inr (refl , <-ascend))

-- grok

Tgr : â„• Ã— â„• â†’ â„• Ã— â„• â†’ ğ’°
Tgr (xâ‚ , xâ‚‚) (yâ‚ , yâ‚‚) = ((xâ‚ â‰¤ yâ‚‚) Ã— (xâ‚‚ < yâ‚‚)) âŠ ((xâ‚‚ < yâ‚) Ã— (xâ‚ < yâ‚))

Rgr : â„• Ã— â„• â†’ â„• Ã— â„• â†’ ğ’°
Rgr (xâ‚ , xâ‚‚) (yâ‚ , yâ‚‚) = (xâ‚ â‰¤ yâ‚) Ã— (xâ‚‚ â‰¤ yâ‚‚)

Tgr-trans : âˆ€ {xâ‚ xâ‚‚ yâ‚ yâ‚‚ zâ‚ zâ‚‚}
          â†’ Tgr (xâ‚ , xâ‚‚) (yâ‚ , yâ‚‚)
          â†’ Tgr (yâ‚ , yâ‚‚) (zâ‚ , zâ‚‚)
          â†’ Tgr (xâ‚ , xâ‚‚) (zâ‚ , zâ‚‚)
Tgr-trans (inl (xâ‚â‰¤yâ‚‚ , xâ‚‚<yâ‚‚)) (inl (_     , yâ‚‚<zâ‚‚)) = inl (xâ‚â‰¤yâ‚‚ âˆ™ <â†’â‰¤ yâ‚‚<zâ‚‚   , <-trans xâ‚‚<yâ‚‚ yâ‚‚<zâ‚‚)
Tgr-trans (inl (xâ‚â‰¤yâ‚‚ , xâ‚‚<yâ‚‚)) (inr (yâ‚‚<zâ‚ , _    )) = inr (<-trans xâ‚‚<yâ‚‚ yâ‚‚<zâ‚ , â‰¤-<-trans xâ‚â‰¤yâ‚‚ yâ‚‚<zâ‚)
Tgr-trans (inr (xâ‚‚<yâ‚ , xâ‚<yâ‚)) (inl (yâ‚â‰¤zâ‚‚ , _    )) = inl (<â†’â‰¤ xâ‚<yâ‚ âˆ™ yâ‚â‰¤zâ‚‚   , <-â‰¤-trans xâ‚‚<yâ‚ yâ‚â‰¤zâ‚‚)
Tgr-trans (inr (xâ‚‚<yâ‚ , xâ‚<yâ‚)) (inr (_     , yâ‚<zâ‚)) = inr (<-trans xâ‚‚<yâ‚ yâ‚<zâ‚ , <-trans xâ‚<yâ‚ yâ‚<zâ‚)

Tgr-empty-intersect : âˆ€ {xâ‚ xâ‚‚ yâ‚ yâ‚‚}
                    â†’ Plus Tgr (xâ‚ , xâ‚‚) (yâ‚ , yâ‚‚)
                    â†’ Rgr (yâ‚ , yâ‚‚) (xâ‚ , xâ‚‚)
                    â†’ âŠ¥
Tgr-empty-intersect p (yâ‰¤xâ‚ , yâ‰¤xâ‚‚) =
  [ (Î» where (_ , x<yâ‚‚) â†’ <â†’â‰± x<yâ‚‚ yâ‰¤xâ‚‚)
  , (Î» where (_ , x<yâ‚) â†’ <â†’â‰± x<yâ‚ yâ‰¤xâ‚)
  ]áµ¤ (plus-fold1 (record { _âˆ™_ = Tgr-trans }) p)

grok : â„• Ã— â„• â†’ â„•
grok =
  to-induction
    (AFâ†’WF (af-Ã— af-â‰¤ af-â‰¤) Tgr-empty-intersect)
    (Î» _ â†’ â„•)
    Î» x ih â†’ go (x .fst) (x .snd) Î» a b â†’ ih (a , b)
  where
  go : âˆ€ x y â†’ (âˆ€ a b â†’ Tgr (a , b) (x , y) â†’ â„•) â†’ â„•
  go  zero    _      _  = 1
  go (suc _)  zero   _  = 1
  go (suc x) (suc y) ih = ih (1 + y) y (inl (refl , <-ascend)) + ih x x (inr (<-ascend , <-ascend))

-- flip1

Tf1 : â„• Ã— â„• â†’ â„• Ã— â„• â†’ ğ’°
Tf1 (xâ‚ , xâ‚‚) (yâ‚ , yâ‚‚) = (xâ‚ â‰¤ yâ‚‚) Ã— (xâ‚‚ < yâ‚)

Rf1 : â„• Ã— â„• â†’ â„• Ã— â„• â†’ ğ’°
Rf1 (xâ‚ , xâ‚‚) (yâ‚ , yâ‚‚) = xâ‚ + xâ‚‚ â‰¤ yâ‚ + yâ‚‚

Tf1-intersection-empty : âˆ€ {xâ‚ xâ‚‚ yâ‚ yâ‚‚}
                       â†’ Plus Tf1 (xâ‚ , xâ‚‚) (yâ‚ , yâ‚‚)
                       â†’ Rf1 (yâ‚ , yâ‚‚) (xâ‚ , xâ‚‚)
                       â†’ âŠ¥
Tf1-intersection-empty {xâ‚} {xâ‚‚} {yâ‚} {yâ‚‚} p yâ‚â‚‚â‰¤xâ‚â‚‚ =
  â‰¤â†’â‰¯ yâ‚â‚‚â‰¤xâ‚â‚‚ $
  plus-fold1 {R = _<_} (record { _âˆ™_ = <-trans}) $
  plus-map (Î» where {a = aâ‚ , aâ‚‚} {b = bâ‚ , bâ‚‚} (aâ‚â‰¤bâ‚‚ , aâ‚‚<bâ‚) â†’
                      subst (aâ‚ + aâ‚‚ <_) (+-comm bâ‚‚ bâ‚) $ â‰¤-<-+ aâ‚â‰¤bâ‚‚ aâ‚‚<bâ‚) p

flip1 : â„• Ã— â„• â†’ â„•
flip1 =
  to-induction
    (AFâ†’WF (af-comap (Î» where (x , y) â†’ x + y) af-â‰¤) Tf1-intersection-empty)
    (Î» _ â†’ â„•)
    Î» x ih â†’ go (x .fst) (x .snd) Î» a b â†’ ih (a , b)
  where
  go : âˆ€ x y â†’ (âˆ€ a b â†’ Tf1 (a , b) (x , y) â†’ â„•) â†’ â„•
  go  zero    _      _  = 1
  go (suc _)  zero   _  = 1
  go (suc x) (suc y) ih = ih (1 + y) x (refl , <-ascend)

-- gnlex

Tgn : â„• Ã— â„• â†’ â„• Ã— â„• â†’ ğ’°
Tgn (xâ‚ , xâ‚‚) (yâ‚ , yâ‚‚) = ((xâ‚ ï¼ yâ‚‚) Ã— (xâ‚‚ < yâ‚‚)) âŠ ((xâ‚ ï¼ yâ‚‚) Ã— (xâ‚‚ < yâ‚))  -- should be collapsed probably

Rgn : â„• Ã— â„• â†’ â„• Ã— â„• â†’ ğ’°
Rgn (xâ‚ , xâ‚‚) (yâ‚ , yâ‚‚) = (xâ‚ â‰¤ yâ‚) Ã— (xâ‚‚ â‰¤ yâ‚‚)

T2-inv : âˆ€ {xâ‚ xâ‚‚ yâ‚ yâ‚‚}
       â†’ pow 2 Tgn (xâ‚ , xâ‚‚) (yâ‚ , yâ‚‚)
       â†’ ((xâ‚ < yâ‚) Ã— (xâ‚‚ < yâ‚)) âŠ ((xâ‚‚ < yâ‚‚) Ã— (xâ‚ < yâ‚‚)) âŠ ((xâ‚ < yâ‚) Ã— (xâ‚‚ < yâ‚‚))
T2-inv ((zâ‚ , zâ‚‚) , inl (exz , x<z) , (wâ‚ , wâ‚‚) , inl (ezw , z<w) , lift ewy) =
  inr $ inl ( <-â‰¤-trans x<z (<â†’â‰¤ z<w âˆ™ =â†’â‰¤ (ap snd ewy))
            , â‰¤-<-trans (=â†’â‰¤ exz) (<-â‰¤-trans z<w (=â†’â‰¤ (ap snd ewy))))
T2-inv ((zâ‚ , zâ‚‚) , inl (exz , x<z) , (wâ‚ , wâ‚‚) , inr (ezw , z<w) , lift ewy) =
  inl       ( â‰¤-<-trans (=â†’â‰¤ exz) (<-â‰¤-trans z<w (=â†’â‰¤ (ap fst ewy)))
            , <-â‰¤-trans x<z (<â†’â‰¤ z<w âˆ™ =â†’â‰¤ (ap fst ewy)))
T2-inv ((zâ‚ , zâ‚‚) , inr (exz , x<z) , (wâ‚ , wâ‚‚) , inl (ezw , z<w) , lift ewy) =
  inr $ inl ( <-â‰¤-trans x<z (=â†’â‰¤ (ezw âˆ™ ap snd ewy))
            , â‰¤-<-trans (=â†’â‰¤ exz) (<-â‰¤-trans z<w (=â†’â‰¤ (ap snd ewy))))
T2-inv ((zâ‚ , zâ‚‚) , inr (exz , x<z) , (wâ‚ , wâ‚‚) , inr (ezw , z<w) , lift ewy) =
  inr $ inr ( â‰¤-<-trans (=â†’â‰¤ exz) (<-â‰¤-trans z<w (=â†’â‰¤ (ap fst ewy)))
            , <-â‰¤-trans x<z (=â†’â‰¤ (ezw âˆ™ ap snd ewy)))

T2-plus-inv : âˆ€ {xâ‚ xâ‚‚ yâ‚ yâ‚‚}
            â†’ Plus (pow 2 Tgn) (xâ‚ , xâ‚‚) (yâ‚ , yâ‚‚)
            â†’ ((xâ‚ < yâ‚) Ã— (xâ‚‚ < yâ‚)) âŠ ((xâ‚‚ < yâ‚‚) Ã— (xâ‚ < yâ‚‚)) âŠ ((xâ‚ < yâ‚) Ã— (xâ‚‚ < yâ‚‚))
T2-plus-inv [ p2 ]âº    = T2-inv p2
T2-plus-inv (_â—…âº_ {y = (wâ‚ , wâ‚‚)} p2 pl) with T2-inv p2 | T2-plus-inv pl
... | inl      (x<wâ‚ , x<wâ‚‚)  | inl      (w<yâ‚ , _   )  = inl       (<-trans x<wâ‚ w<yâ‚ , <-trans x<wâ‚‚ w<yâ‚)
... | inl      (x<wâ‚ , x<wâ‚‚)  | inr (inl (_    , w<yâ‚)) = inr $ inl (<-trans x<wâ‚‚ w<yâ‚ , <-trans x<wâ‚ w<yâ‚)
... | inl      (x<wâ‚ , x<wâ‚‚)  | inr (inr (w<yâ‚ , _   )) = inl       (<-trans x<wâ‚ w<yâ‚ , <-trans x<wâ‚‚ w<yâ‚)
... | inr (inl (x<wâ‚‚ , x<wâ‚)) | inl      (_    , w<yâ‚‚)  = inl       (<-trans x<wâ‚ w<yâ‚‚ , <-trans x<wâ‚‚ w<yâ‚‚)
... | inr (inl (x<wâ‚‚ , x<wâ‚)) | inr (inl (w<yâ‚‚ , _   )) = inr $ inl (<-trans x<wâ‚‚ w<yâ‚‚ , <-trans x<wâ‚ w<yâ‚‚)
... | inr (inl (x<wâ‚‚ , x<wâ‚)) | inr (inr (_    , w<yâ‚‚)) = inr $ inl (<-trans x<wâ‚‚ w<yâ‚‚ , <-trans x<wâ‚ w<yâ‚‚)
... | inr (inr (x<wâ‚ , x<wâ‚‚)) | inl      (w<yâ‚ , w<yâ‚‚)  = inl       (<-trans x<wâ‚ w<yâ‚ , <-trans x<wâ‚‚ w<yâ‚‚)
... | inr (inr (x<wâ‚ , x<wâ‚‚)) | inr (inl (w<yâ‚‚ , w<yâ‚)) = inr $ inl (<-trans x<wâ‚‚ w<yâ‚‚ , <-trans x<wâ‚ w<yâ‚)
... | inr (inr (x<wâ‚ , x<wâ‚‚)) | inr (inr (w<yâ‚ , w<yâ‚‚)) = inr $ inr (<-trans x<wâ‚ w<yâ‚ , <-trans x<wâ‚‚ w<yâ‚‚)

Tgn-plus-decompose : âˆ€ {xâ‚ xâ‚‚ yâ‚ yâ‚‚}
                   â†’ Plus Tgn (xâ‚ , xâ‚‚) (yâ‚ , yâ‚‚)
                   â†’ Tgn (xâ‚ , xâ‚‚) (yâ‚ , yâ‚‚)
                   âŠ Plus (pow 2 Tgn) (xâ‚ , xâ‚‚) (yâ‚ , yâ‚‚)
                   âŠ (Î£[ (zâ‚ , zâ‚‚) ê‰ â„• Ã— â„• ] (Tgn (xâ‚ , xâ‚‚) (zâ‚ , zâ‚‚)) Ã— (Plus (pow 2 Tgn) (zâ‚ , zâ‚‚) (yâ‚ , yâ‚‚)))
Tgn-plus-decompose                     [ txy ]âº                       = inl txy
Tgn-plus-decompose {xâ‚} {xâ‚‚} {yâ‚} {yâ‚‚} (_â—…âº_ {y = (wâ‚ , wâ‚‚)} txw pwy) with Tgn-plus-decompose pwy
... | inl twy                           = inr $ inl [ (wâ‚ , wâ‚‚) , txw , (yâ‚ , yâ‚‚) , twy , lift refl ]âº
... | inr (inl p)                       = inr $ inr ((wâ‚ , wâ‚‚) , txw , p)
... | inr (inr ((zâ‚ , zâ‚‚) , twz , pzy)) = inr $ inl (((wâ‚ , wâ‚‚) , txw , (zâ‚ , zâ‚‚) , twz , lift refl) â—…âº pzy)

Tgn-empty-intersect : âˆ€ {xâ‚ xâ‚‚ yâ‚ yâ‚‚}
                    â†’ Plus Tgn (xâ‚ , xâ‚‚) (yâ‚ , yâ‚‚)
                    â†’ Rgn (yâ‚ , yâ‚‚) (xâ‚ , xâ‚‚)
                    â†’ âŠ¥
Tgn-empty-intersect p (yâ‰¤xâ‚ , yâ‰¤xâ‚‚) =
  [ (Î» where
         (inl (e , xâ‚‚<yâ‚‚)) â†’ <â†’â‰± xâ‚‚<yâ‚‚ yâ‰¤xâ‚‚
         (inr (e , xâ‚‚<yâ‚)) â†’ <â†’â‰± xâ‚‚<yâ‚ (yâ‰¤xâ‚ âˆ™ =â†’â‰¤ e âˆ™ yâ‰¤xâ‚‚))
  , [ [ (Î» where (xâ‚<yâ‚ , _) â†’ <â†’â‰± xâ‚<yâ‚ yâ‰¤xâ‚)
      , [ (Î» where (xâ‚‚<yâ‚‚ , _) â†’ <â†’â‰± xâ‚‚<yâ‚‚ yâ‰¤xâ‚‚)
        , (Î» where (xâ‚<yâ‚ , _) â†’ <â†’â‰± xâ‚<yâ‚ yâ‰¤xâ‚)
        ]áµ¤
      ]áµ¤ âˆ˜ T2-plus-inv
    , (Î» where ((zâ‚ , zâ‚‚) , txz , pzy) â†’
                  [ [ (Î» where (e , _) (_ , zâ‚‚<yâ‚) â†’ <â†’â‰± zâ‚‚<yâ‚ (yâ‰¤xâ‚ âˆ™ =â†’â‰¤ e))
                    , (Î» where (e , _) (_ , zâ‚‚<yâ‚) â†’ <â†’â‰± zâ‚‚<yâ‚ (yâ‰¤xâ‚ âˆ™ =â†’â‰¤ e))
                    ]áµ¤ txz
                  , [ (Î» where
                           (_ , xâ‚‚<zâ‚‚) (inl (zâ‚‚<yâ‚‚ , _    )) â†’ â‰¤â†’â‰¯ yâ‰¤xâ‚‚ (<-trans xâ‚‚<zâ‚‚ zâ‚‚<yâ‚‚)
                           (_ , xâ‚‚<zâ‚‚) (inr (_     , zâ‚‚<yâ‚‚)) â†’ â‰¤â†’â‰¯ yâ‰¤xâ‚‚ (<-trans xâ‚‚<zâ‚‚ zâ‚‚<yâ‚‚))
                    , (Î» where
                           (_ , xâ‚‚<zâ‚) (inl (_     , zâ‚<yâ‚‚)) â†’ â‰¤â†’â‰¯ yâ‰¤xâ‚‚ (<-trans xâ‚‚<zâ‚ zâ‚<yâ‚‚)
                           (e , xâ‚‚<zâ‚) (inr (zâ‚<yâ‚ , zâ‚‚<yâ‚‚)) â†’ â‰¤â†’â‰¯ (yâ‰¤xâ‚ âˆ™ =â†’â‰¤ e) (<-trans zâ‚‚<yâ‚‚ (â‰¤-<-trans yâ‰¤xâ‚‚ (<-trans xâ‚‚<zâ‚ zâ‚<yâ‚))))
                    ]áµ¤ txz
                  ]áµ¤ (T2-plus-inv pzy))
    ]áµ¤
  ]áµ¤ (Tgn-plus-decompose p)

gnlex : â„• Ã— â„• â†’ â„•
gnlex =
  to-induction
    (AFâ†’WF (af-Ã— af-â‰¤ af-â‰¤) Tgn-empty-intersect)
    (Î» _ â†’ â„•)
    Î» x ih â†’ go (x .fst) (x .snd) Î» a b â†’ ih (a , b)
  where
  go : âˆ€ x y â†’ (âˆ€ a b â†’ Tgn (a , b) (x , y) â†’ â„•) â†’ â„•
  go  zero    _      _  = 1
  go (suc _)  zero   _  = 1
  go (suc x) (suc y) ih = ih (1 + y) y (inl (refl , <-ascend)) + ih (1 + y) x (inr (refl , <-ascend))

{-
-- fsum

Tfs : â„• âŠ â„• â†’ â„• âŠ â„• â†’ ğ’°
Tfs x y = (Î£[ z ê‰ â„• ] (x ï¼ inr (2 + z)) Ã— (y ï¼ inl (1 + z)))
        âŠ (Î£[ z ê‰ â„• ] (x ï¼ inl (z âˆ¸ 2)) Ã— (y ï¼ inr z))

Rfs : â„• âŠ â„• â†’ â„• âŠ â„• â†’ ğ’°
Rfs = â†‘âŠ _â‰¤_ _â‰¤_

fsum : â„• âŠ â„• â†’ â„•
fsum =
  to-induction
    (AFâ†’WF {R = Rfs} {T = Tfs}
           (af-âŠ af-â‰¤ af-â‰¤)
           {!!})
    (Î» _ â†’ â„•)
    go
  where
  go : (x : â„• âŠ â„•) â†’ ((y : â„• âŠ â„•) â†’ Tfs y x â†’ â„•) â†’ â„•
  go (inl zero)    ih = 1
  go (inl (suc x)) ih = ih (inr (2 + x)) (inl (x , (refl , refl)))
  go (inr x)       ih = ih (inl (x âˆ¸ 2)) (inr (x , (refl , refl)))
-}

