{-# OPTIONS --safe #-}
module Data.Acc.Properties where

open import Meta.Prelude
open Variadics _

open import Data.Acc.Base
open import Data.Empty.Base

private variable
  â„“a â„“b â„“ â„“â€² : Level
  A : ğ’° â„“a
  B : ğ’° â„“b
  _<_ _<â€²_ : A â†’ A â†’ ğ’° â„“

acc-lift : (f : B â†’ A) (b : B)
         â†’ Acc _<_ (f b) â†’ Acc (Î» x y â†’ f x < f y) b
acc-lift f b (acc rec) = acc Î» y p â†’ acc-lift f y (rec (f y) p)


-- well-foundedness

wfâ†’irrefl : is-wf _<_ â†’ âˆ€ x â†’ Â¬ x < x
wfâ†’irrefl {_<_} wf = to-induction wf (Î» z â†’ Â¬ z < z)
  Î» x ih x<x â†’ ih x x<x x<x

is-wfâ†’asym : is-wf _<_ â†’ âˆ€ x y â†’ x < y â†’ Â¬ y < x
is-wfâ†’asym {_<_} wf = to-induction wf (Î» z â†’ âˆ€ y â†’ z < y â†’ Â¬ y < z)
  Î» x ih y x<y y<x â†’ ih y y<x x y<x x<y

wf-map : {_<_ : A â†’ A â†’ ğ’° â„“} {_<â€²_ : A â†’ A â†’ ğ’° â„“â€²}
       â†’ Î [ _<â€²_ â‡’ _<_ ]
       â†’ is-wf _<_ â†’ is-wf _<â€²_
wf-map {_<â€²_} h wf =
  to-induction wf (Acc _<â€²_)
    Î» x ih â†’ acc Î» y y<â€²x â†’ ih y (h y x y<â€²x)

wf-lift : (f : B â†’ A)
        â†’ is-wf _<_ â†’ is-wf (Î» x y â†’ f x < f y)
wf-lift f wf x = acc-lift f x (wf (f x))


-- Noetherianness

noethâ†’irrefl : is-noeth _<_ â†’ âˆ€ x â†’ Â¬ x < x
noethâ†’irrefl {_<_} nth =
  to-ninduction nth (Î» z â†’ Â¬ z < z)
    Î» x ih x<x â†’ ih x x<x x<x

noethâ†’asym : is-noeth _<_ â†’ âˆ€ x y â†’ x < y â†’ Â¬ y < x
noethâ†’asym {_<_} nth =
  to-ninduction nth (Î» z â†’ âˆ€ y â†’ z < y â†’ Â¬ y < z)
    Î» x ih y x<y y<x â†’ ih y x<y x y<x x<y

noeth-map : {_<_ : A â†’ A â†’ ğ’° â„“} {_<â€²_ : A â†’ A â†’ ğ’° â„“â€²}
          â†’ Î [ _<â€²_ â‡’ _<_ ]
          â†’ is-noeth _<_ â†’ is-noeth _<â€²_
noeth-map {_<â€²_} h nth =
  to-ninduction nth (Acc (flip _<â€²_))
    Î» x ih â†’ acc Î» y x<â€²y â†’ ih y (h x y x<â€²y)

noeth-lift : (f : B â†’ A)
           â†’ is-noeth _<_ â†’ is-noeth (Î» x y â†’ f x < f y)
noeth-lift f nth x = acc-lift f x (nth (f x))


-- finite height

finite-height-lift
  : (f : B â†’ A)
  â†’ is-of-finite-height _<_ â†’ is-of-finite-height (Î» x y â†’ f x < f y)
finite-height-lift f fh x = acc-lift f x (fh (f x) .fst) , acc-lift f x (fh (f x) .snd)
