{-# OPTIONS --safe #-}
module Data.Nat.DivMod where

open import Foundations.Base
open import Foundations.Equiv
open import Meta.Marker
open import Data.Nat.Base renaming (div-helper to divâ‚•; mod-helper to modâ‚•)
open import Data.Nat.Path
open import Data.Nat.Order.Inductive
open import Data.Empty.Base
open import Data.Sum.Base
open import Data.Nat.Properties

infix 4 _âˆ£_
infixl 7 _/_
infixl 7 _%_

-- division (rounding down)

_/_ : â„• â†’ â„• â†’ â„•
m /  zero   = 0
m / (suc n) = divâ‚• 0 n m n

-- modulo

_%_ : â„• â†’ â„• â†’ â„•
m %  zero   = m
m % (suc n) = modâ‚• 0 n m n

-- divisibility

record _âˆ£_ (m n : â„•) : ğ’° where
  constructor divides
  field quot  : â„•
        proof : n ï¼ quot Â· m

-- properties

0-div-0 : âˆ€ n â†’ 0 / n ï¼ 0
0-div-0  zero   = refl
0-div-0 (suc n) = refl

div-mod-lemma : âˆ€ am ad d n
              â†’ am + ad Â· suc (am + n) + d ï¼ modâ‚• am (am + n) d n + divâ‚• ad (am + n) d n Â· suc (am + n)
div-mod-lemma am ad  zero    n      = +-zero-r (am + ad Â· suc (am + n))
div-mod-lemma am ad (suc d)  zero   =
    ap (Î» q â†’ am + ad Â· suc q + suc d) (+-zero-r am)
  âˆ™ +-suc-r (am + ad Â· suc am) d
  âˆ™ div-mod-lemma 0 (suc ad) d am
  âˆ™ ap (Î» q â†’ modâ‚• 0 q d q + divâ‚• (suc ad) q d q Â· suc q) (sym $ +-zero-r am)
div-mod-lemma am ad (suc d) (suc n) =
    ap (Î» q â†’ am + ad Â· suc q + suc d) (+-suc-r am n)
  âˆ™ +-suc-r (am + ad Â· suc (suc (am + n))) d
  âˆ™ div-mod-lemma (suc am) ad d n
  âˆ™ ap (Î» q â†’ modâ‚• (suc am) q d n + divâ‚• ad q d n Â· suc q) (sym $ +-suc-r am n)

modâ‚•-skipTo0 : âˆ€ acc n a b â†’ modâ‚• acc n (b + a) a ï¼ modâ‚• (a + acc) n b 0
modâ‚•-skipTo0 acc n  zero   b = ap (Î» q â†’ modâ‚• acc n q 0) (+-zero-r b)
modâ‚•-skipTo0 acc n (suc a) b =
    ap (Î» q â†’ modâ‚• acc n q (suc a)) (+-suc-r b a)
  âˆ™ modâ‚•-skipTo0 (suc acc) n a b
  âˆ™ ap (Î» q â†’ modâ‚• q n b 0) (+-suc-r a acc)

n[modâ‚•]nâ‰¡0 : âˆ€ acc v â†’ modâ‚• acc (acc + v) (suc v) v ï¼ 0
n[modâ‚•]nâ‰¡0 acc v = modâ‚•-skipTo0 acc (acc + v) v 1

aâ‰¤nâ‡’a[modâ‚•]nâ‰¡a : âˆ€ acc n a b â†’ modâ‚• acc n a (a + b) ï¼ acc + a
aâ‰¤nâ‡’a[modâ‚•]nâ‰¡a acc n  zero   b = sym (+-zero-r acc)
aâ‰¤nâ‡’a[modâ‚•]nâ‰¡a acc n (suc a) b = aâ‰¤nâ‡’a[modâ‚•]nâ‰¡a (suc acc) n a b âˆ™ sym (+-suc-r acc a)

mâ‰¡m%n+[m/n]*n : âˆ€ m n â†’ m ï¼ m % n + (m / n) Â· n
mâ‰¡m%n+[m/n]*n m  zero   = sym $ +-zero-r m
mâ‰¡m%n+[m/n]*n m (suc n) = div-mod-lemma 0 0 m n

m%nâ‰¡mâˆ¸m/n*n : âˆ€ m n â†’ m % n ï¼ m âˆ¸ (m / n) Â· n
m%nâ‰¡mâˆ¸m/n*n m n =
  m % n
    ï¼Ë˜âŸ¨ +-cancel-âˆ¸-r (m % n) ((m / n) Â· n ) âŸ©
  m % n + m / n Â· n âˆ¸ m / n Â· n
    ï¼Ë˜âŸ¨ ap (_âˆ¸ m / n Â· n) (mâ‰¡m%n+[m/n]*n m n) âŸ©
  m âˆ¸ (m / n) Â· n
    âˆ

[m/n]*nï¼ : âˆ€ m n â†’ (m / n) Â· n ï¼ m âˆ¸ m % n
[m/n]*nï¼ m n = sym (+-cancel-âˆ¸-r (m / n Â· n) (m % n))
              âˆ™ ap (_âˆ¸ m % n) (+-comm (m / n Â· n) (m % n) âˆ™ sym (mâ‰¡m%n+[m/n]*n m n))

n%nï¼0 : âˆ€ n â†’ n % n ï¼ 0
n%nï¼0  zero   = refl
n%nï¼0 (suc n) = n[modâ‚•]nâ‰¡0 0 n

âˆ£-is-prop : âˆ€ m n â†’ m â‰  0 â†’ is-prop (m âˆ£ n)
âˆ£-is-prop m n mâ‰ 0 = is-prop-Î· go
  where
  go : (p q : m âˆ£ n) â†’ p ï¼ q
  go (divides qâ‚ prfâ‚) (divides qâ‚‚ prfâ‚‚) =
    apÂ² divides
      ([ id , (Î» m=0 â†’ absurd (mâ‰ 0 m=0)) ]áµ¤ (Â·-cancel-r qâ‚ qâ‚‚ m (sym prfâ‚ âˆ™ prfâ‚‚)))
      (to-pathá´¾ (is-set-Î² â„•-is-set n _ _ prfâ‚‚))

Â¬0âˆ£suc : âˆ€ n â†’ Â¬ (0 âˆ£ suc n)
Â¬0âˆ£suc n (divides q pf) = absurd (sucâ‰ zero (pf âˆ™ Â·-absorb-r q))

âˆ£â†’â‰¤ : âˆ€ m n â†’ n â‰  0 â†’ m âˆ£ n â†’ m â‰¤ n
âˆ£â†’â‰¤ m    zero     nâ‰ 0  mn                  = absurd (nâ‰ 0 refl)
âˆ£â†’â‰¤ m   (suc n)   nâ‰ 0 (divides  zero   pf) = absurd (sucâ‰ zero pf)
âˆ£â†’â‰¤ m n@(suc n-1) nâ‰ 0 (divides (suc q) pf) = â‰¤-trans â‰¤-+-r (subst (_â‰¤ n) pf â‰¤-refl)

âˆ£-refl : âˆ€ n â†’ n âˆ£ n
âˆ£-refl n = divides 1 (sym $ Â·-id-l n)

âˆ£-trans : âˆ€ m n p â†’ m âˆ£ n â†’ n âˆ£ p â†’ m âˆ£ p
âˆ£-trans m n p (divides qm prfm) (divides qn prfn) =
  divides (qn Â· qm) (prfn âˆ™ ap (qn Â·_) prfm âˆ™ Â·-assoc qn qm m)

âˆ£-antisym : âˆ€ m n â†’ m âˆ£ n â†’ n âˆ£ m â†’ m ï¼ n
âˆ£-antisym  zero    n     (divides q prf) nâˆ£m = sym (prf âˆ™ Â·-absorb-r q)
âˆ£-antisym (suc m)  zero   mâˆ£n            nâˆ£m = absurd (Â¬0âˆ£suc m nâˆ£m)
âˆ£-antisym (suc m) (suc n) mâˆ£n            nâˆ£m =
  â‰¤-antisym (âˆ£â†’â‰¤ (suc m) (suc n) sucâ‰ zero mâˆ£n) (âˆ£â†’â‰¤ (suc n) (suc m) sucâ‰ zero nâˆ£m)

_âˆ£0 : âˆ€ n â†’ n âˆ£ 0
n âˆ£0 = divides 0 refl

âˆ£nâˆ£m%nâ‡’âˆ£m : âˆ€ {m n d} â†’ d âˆ£ n â†’ d âˆ£ m % n â†’ d âˆ£ m
âˆ£nâˆ£m%nâ‡’âˆ£m {m} {n} {d} (divides q prf) (divides qm prfm) =
  divides (qm + (m / n) Â· q)
    (m
      ï¼âŸ¨ mâ‰¡m%n+[m/n]*n m n âŸ©
     âŒœ m % n âŒ + m / n Â· n
      ï¼âŸ¨ ap! prfm âŸ©
     qm Â· d + m / n Â· âŒœ n âŒ
      ï¼âŸ¨ ap! prf âŸ©
     qm Â· d + âŒœ m / n Â· (q Â· d) âŒ
      ï¼âŸ¨ ap! (Â·-assoc (m / n) q d) âŸ©
     qm Â· d + m / n Â· q Â· d
      ï¼Ë˜âŸ¨ Â·-distrib-+-r qm (m / n Â· q) d âŸ©
    (qm + m / n Â· q) Â· d
      âˆ)

%-presË¡-âˆ£ : âˆ€ {m n d} â†’ d âˆ£ m â†’ d âˆ£ n â†’ d âˆ£ m % n
%-presË¡-âˆ£ {m} {n} {d} (divides qm prfm) (divides qn prfn) =
  divides (qm âˆ¸ m / n Â· qn)
    (m % n
       ï¼âŸ¨ m%nâ‰¡mâˆ¸m/n*n m n âŸ©
     m âˆ¸ m / n Â· âŒœ n âŒ
       ï¼âŸ¨ ap! prfn âŸ©       
     m âˆ¸ âŒœ m / n Â· (qn Â· d) âŒ
       ï¼âŸ¨ ap! (Â·-assoc (m / n) qn d) âŸ©       
     âŒœ m âŒ âˆ¸ m / n Â· qn Â· d
       ï¼âŸ¨ ap! prfm âŸ©       
     qm Â· d âˆ¸ m / n Â· qn Â· d
       ï¼Ë˜âŸ¨ Â·-distrib-âˆ¸-r qm (m / n Â· qn) d âŸ©       
     (qm âˆ¸ m / n Â· qn) Â· d
       âˆ)
